test/rewrite_search.lean
@@ -1,0 +1,37 @@
+import tidy.rewrite_search
+
+namespace tidy.test
+
+open tactic.interactive
+
+@[ematch] private axiom foo : [0] = [1]
+@[ematch] private axiom bar1 : [1] = [2]
+@[ematch] private axiom bar2 : [3] = [2]
+@[ematch] private axiom bar3 : [3] = [4]
+
+private example : [[0],[0]] = [[4],[4]] :=
+begin
+rewrite_search [foo, bar1, ← bar2, bar2, ← bar3],
+end
+
+private example : [[0],[0]] = [[4],[4]] :=
+begin
+rewrite_search_using `ematch,
+end
+
+private axiom qux : [[0],[0]] = [[4],[5]]
+
+private example : [[0],[0]] = [[4],[5]] :=
+begin
+success_if_fail { rewrite_search_using `ematch },
+exact qux
+end
+
+@[ematch] private axiom foo' (n : ℕ) : [n, n] = [n+1, n+1]
+
+private example : [0,0] = [1,1] :=
+begin
+rewrite_search_using `ematch,
+end
+
+end tidy.test
